## Penyelesaian Turunan Fungsi

### 1. Bila $f(x) = (x^2 + 1)^2$, tentukan $f'(x)$.


$f(x) = (x^2 + 1)^2$


$f'(x) = 2(x^2+1)\cdot(2x)$


$f'(x) = 4x(x^2+1)$

---

### 2. Diketahui $g(x) = 3x(x^3 - 1)$, tentukan $g''(x)$.


$g(x) = 3x(x^3 - 1) = 3x^4 - 3x$


$g'(x) = 12x^3 - 3$


$g''(x) = 36x^2$

---

### 3. Diketahui $h(x) = \dfrac{3x - 5}{x^2 + 7}$, tentukan $h'(-1)$.

Rumus turunan hasil bagi:


$h'(x) = \frac{u'v - uv'}{v^2}, \quad u = 3x-5, \ v = x^2+7$


$h'(x) = \frac{3(x^2+7) - (3x-5)(2x)}{(x^2+7)^2}$


$= \frac{3x^2 + 21 - 6x^2 + 10x}{(x^2+7)^2}$


$= \frac{-3x^2 + 10x + 21}{(x^2+7)^2}$

Substitusi $x = -1:$


$h'(-1) = \frac{-3(-1)^2 + 10(-1) + 21}{((-1)^2+7)^2}$


$= \frac{-3 - 10 + 21}{64}$


$= \frac{8}{64} = \frac{1}{8}$

---

### **Kesimpulan**


$f'(x) = 4x(x^2+1), \quad g''(x) = 36x^2, \quad h'(-1) = \tfrac{1}{8}$
